byteback-test/test-java-17/src/main/java/byteback/test/patternmatching/Basic.java
@@ -1,8 +1,16 @@
+/**
+ * RUN: %{byteback} -cp %{jar} -c %{class} -o %t.bpl
+ */
+
 package byteback.test.patternmatching;
+
+import static byteback.specification.Contract.assertion;
+
+import java.util.ArrayList;
 
 public class Basic {
 
-	public static int test() {
+	public static int Convert_ArrayPatternMatch() {
 		Object obj = new int[10];
 
 		if (obj instanceof int[] matched) {
@@ -14,4 +22,48 @@ public class Basic {
 		return 0;
 	}
 
+	public static int Convert_InstancePatternMatch() {
+		Object obj = new ArrayList<>();
+
+		if (obj instanceof ArrayList matched) {
+			int size = matched.size();
+
+			return size;
+		}
+
+		return 0;
+	}
+
+	public static int AssertFalse_InUnreachableMatchIf_Verifies() {
+		Object obj = new Object();
+
+		if (obj instanceof ArrayList matched) {
+			int size = matched.size();
+			assertion(false);
+
+			return size;
+		}
+
+		return 0;
+	}
+
+	public static int AssertFalse_InReachableMatchIf_Fails() {
+		Object obj = new ArrayList<>();
+
+		if (obj instanceof ArrayList matched) {
+			int size = matched.size();
+			// CHECK: Error: this assertion could not be proved
+			assertion(false);
+
+			return size;
+		}
+
+		return 0;
+	}
+
 }
+
+/**
+ * RUN: %{verify} %t.bpl | filecheck %s
+ * CHECK: Boogie program verifier finished with 4 verified, 1 error
+ */
